order

specs/ecdsap256/Spec.ECDSA.fst
@@ -270,8 +270,7 @@ unfold let prime_order_inverse_list (#c: curve) : list uint8 =
    ]
 
 
-let prime_p256_order_inverse_seq (#c: curve) : (s:lseq uint8 (getCoordinateLen c) {nat_from_intseq_le s == (getPrimeOrder #c) - 2}) =
-  let order = getPrimeOrder #c in 
+let prime_p256_order_inverse_seq (#c: curve) : (s:lseq uint8 (getCoordinateLen c) {nat_from_intseq_le s == getPrimeOrder #c - 2}) =  
   assert_norm (List.Tot.length (prime_order_inverse_list #P256) == getCoordinateLen P256);
   assert_norm (List.Tot.length (prime_order_inverse_list #P384) == getCoordinateLen P384);
   nat_from_intlist_seq_le (getCoordinateLen c) (prime_order_inverse_list #c); 
@@ -279,23 +278,36 @@ let prime_p256_order_inverse_seq (#c: curve) : (s:lseq uint8 (getCoordinateLen c
   assert_norm (nat_from_intlist_le (prime_order_inverse_list #P384) == getPrimeOrder #P384 - 2);
   of_list (prime_order_inverse_list #c)
 
-    
+
+unfold let prime_order_list (#c: curve) : list uint8 =
+  match c with 
+  |P256 -> 
+    [
+      u8 255; u8 255; u8 255; u8 255; u8 0;   u8 0;   u8 0;   u8 0;
+      u8 255; u8 255; u8 255; u8 255; u8 255; u8 255; u8 255; u8 255;
+      u8 188; u8 230; u8 250; u8 173; u8 167; u8 23;  u8 158; u8 132;
+      u8 243; u8 185; u8 202; u8 194; u8 252; u8 99;  u8 37;  u8 81
+    ]
+  |P384 -> 
+    [
+      u8 255; u8 255; u8 255; u8 255; u8 255; u8 255; u8 255; u8 255;
+      u8 255; u8 255; u8 255; u8 255; u8 255; u8 255; u8 255; u8 255;
+      u8 255; u8 255; u8 255; u8 255; u8 255; u8 255; u8 255; u8 255;
+      u8 199; u8 99;  u8 77;  u8 129; u8 244; u8 55;  u8 45;  u8 223;
+      u8 88;  u8 26;  u8 13;  u8 178; u8 72 ; u8 176; u8 167; u8 122;
+      u8 236; u8 236; u8 25;  u8 106; u8 204; u8 197; u8 41;  u8 115
+    ]
 
 
-unfold let prime_p256_order_list: list uint8 =
- [
-  u8 255; u8 255; u8 255; u8 255; u8 0;  u8 0;   u8 0;   u8 0;
-  u8 255; u8 255; u8 255; u8 255; u8 255; u8 255; u8 255; u8 255;
-  u8 188; u8 230; u8 250; u8 173; u8 167; u8 23; u8 158; u8 132;
-  u8 243; u8 185; u8 202; u8 194; u8 252; u8 99; u8 37; u8 81
- ]
-
-
-let prime_p256_order_seq: s:lseq uint8 32{nat_from_intseq_be s == prime_p256_order} =
-  assert_norm (List.Tot.length prime_p256_order_list == 32);
-  nat_from_intlist_seq_be 32 prime_p256_order_list;
-  assert_norm (nat_from_intlist_be prime_p256_order_list == prime_p256_order);
-  of_list prime_p256_order_list
+let prime_p256_order_seq (#c: curve) : s:lseq uint8 (getCoordinateLen c) 
+  {nat_from_intseq_be s == (getPrimeOrder #c)} =
+  assert_norm (List.Tot.length (prime_order_list #P256) == getCoordinateLen P256);
+  assert_norm (List.Tot.length (prime_order_list #P384) == getCoordinateLen P384);
+  nat_from_intlist_seq_be (getCoordinateLen P256) (prime_order_list #P256);
+  nat_from_intlist_seq_be (getCoordinateLen P384) (prime_order_list #P384); 
+  assert_norm (nat_from_intlist_be (prime_order_list #P256) == getPrimeOrder #P256);
+  assert_norm (nat_from_intlist_be (prime_order_list #P384) == getPrimeOrder #P384);
+  of_list (prime_order_list #c)
 
 
 val exponent_spec: a:nat_prime -> r:nat_prime{r = pow a (prime_p256_order - 2) % prime_p256_order}
